Reducing Interpolants to minor sorrys

GL/Interpolants.lean
@@ -3,6 +3,8 @@ import GL.CoalgebraProof
 import GL.SplitCoalgebraProof
 import Mathlib.Data.Fintype.Defs
 import GL.Semantics
+import GL.FixedPointTheorem
+import GL.AxiomBlame
 
 namespace Split
 
@@ -23,8 +25,8 @@ theorem at_in_lt_freeVar {𝕏 : Proof} [fin_X : Fintype 𝕏.X] {n : Nat} (h : 
 noncomputable def encodeVar {𝕏 : Proof} [Fintype 𝕏.X] : 𝕏.X → Nat :=
   fun x ↦ 𝕏.freeVar + Fintype.equivFin 𝕏.X x
 
-noncomputable def unencodeVar {𝕏 : Proof} [Fintype 𝕏.X] (n : Nat) (h : n - 𝕏.freeVar < Fintype.card 𝕏.X) : 𝕏.X :=
-  (Fintype.equivFin 𝕏.X).symm ⟨n - 𝕏.freeVar, h⟩
+noncomputable def unencodeVar {𝕏 : Proof} [Fintype 𝕏.X] (n : Nat) (h1 : n - 𝕏.freeVar < Fintype.card 𝕏.X) : 𝕏.X :=
+  (Fintype.equivFin 𝕏.X).symm ⟨n - 𝕏.freeVar, h1⟩
 
 lemma encodeVar_inj (𝕏 : Proof) [Fintype 𝕏.X] : Function.Injective (@encodeVar 𝕏 _) := by
   simp [Function.Injective]
@@ -32,8 +34,16 @@ lemma encodeVar_inj (𝕏 : Proof) [Fintype 𝕏.X] : Function.Injective (@encod
   simp [encodeVar, Fin.val_eq_val] at hyp
   exact hyp
 
+@[simp] -- the other version using Function.Injective does not work well with simp
+lemma encodeVar_inj' (𝕏 : Proof) [Fintype 𝕏.X] (x y : 𝕏.X) : @encodeVar 𝕏 _ x = @encodeVar 𝕏 _ y ↔ x = y := by
+  simp [encodeVar, Fin.val_eq_val]
+
 lemma encodeVar_inv (𝕏 : Proof) [Fintype 𝕏.X] (x : 𝕏.X) : unencodeVar (encodeVar x) (by simp [encodeVar]) = x := by
   simp [unencodeVar, encodeVar]
+
+lemma unencodeVar_inv (𝕏 : Proof) [Fintype 𝕏.X] (n : ℕ) (h1) (h2 : n ≥ 𝕏.freeVar) : encodeVar (@unencodeVar 𝕏 _ n h1) = n := by
+  simp [unencodeVar, encodeVar]
+  omega
 
 lemma at_in_not_encodeVar {𝕏 : Proof} [fin_X : Fintype 𝕏.X] {n : Nat} (h : at n ∈ 𝕏.Sequent) (x : 𝕏.X) : ¬ encodeVar x = n := by
   have := at_in_lt_freeVar h
@@ -84,8 +94,6 @@ theorem partial_const {p : Nat → Prop} [DecidablePred p] (σ : Subtype p → F
   induction A <;> simp_all [partial_, Formula.instTop, Formula.instBot, not_true_eq_false, Formula.vocab, -not_and, not_and_or]
   all_goals
     aesop
-
-#check Finset.instInsert
 @[simp]
 theorem Finset.doubleton_subset_iff {α : Type} [DecidableEq α] {s : Finset α} {a b : α} : {a, b} ⊆ s ↔ a ∈ s ∧ b ∈ s := by simp [Finset.subset_iff]
 
@@ -97,7 +105,7 @@ theorem extend_in {𝕏 : Proof} [fin_X : Fintype 𝕏.X] {Y : Finset 𝕏.X} (Y
   all_goals
     aesop
 
-theorem encodeVar_in_equation_imp_pred {𝕏 : Proof} [fin_X : Fintype 𝕏.X] {x y : 𝕏.X} :
+theorem encodeVar_in_equation_imp_edge {𝕏 : Proof} [fin_X : Fintype 𝕏.X] {x y : 𝕏.X} :
   encodeVar y ∈ (equation x).vocab → (edge 𝕏.α) x y := by
   unfold equation
   split <;> simp [Formula.vocab, encodeVar, ←Fin.ext_iff, edge]
@@ -117,6 +125,22 @@ theorem encodeVar_in_equation_imp_pred {𝕏 : Proof} [fin_X : Fintype 𝕏.X] {
     linarith
   all_goals
     aesop
+
+def SplitSequent.left (Γ : SplitSequent) : Sequent := Γ.filterMap (Sum.getLeft?) (by aesop)
+def SplitSequent.right (Γ : SplitSequent) : Sequent := Γ.filterMap (Sum.getRight?) (by aesop)
+
+theorem var_in_equation {𝕏 : Proof} [fin_X : Fintype 𝕏.X] {x : 𝕏.X} (n : ℕ) :
+  n ∈ (equation x).vocab → n ∈ (SplitSequent.left (f (r 𝕏.α x))).vocab ∩ (SplitSequent.right (f (r 𝕏.α x))).vocab
+  ∨ ∃ y, encodeVar y = n ∧ (edge 𝕏.α) x y := by
+  unfold equation
+  split <;> simp [Formula.vocab, encodeVar, edge] <;> try grind
+  case h_4 Δ n in_Δ r =>  -- this is a contradiction because it cannot be = n
+    simp [r, f, SplitSequent.left, SplitSequent.right, Sequent.vocab]
+    grind [Formula.vocab]
+  case h_5 Δ n in_Δ r =>
+    simp [r, f, SplitSequent.left, SplitSequent.right, Sequent.vocab]
+    grind [Formula.vocab]
+
 
 theorem single_preserves_equiv (n : Nat) (C D E : Formula) (h : D ≅ E) : single n C D ≅ single n C E := by
   induction D <;> induction E <;> simp [single] <;> try exact h
@@ -225,7 +249,18 @@ def Solution_strong {𝕏 : Proof} [fin_X : Fintype 𝕏.X]
       have box_in_Y := exists_box_on_restr_loop loop_con.choose (fun x ↦ x ∈ Y) loop_con.choose_spec
       let box := box_in_Y.choose
       have τ := @Solution_strong _ _ (Y \ {box}) (by simp [Finset.subset_iff]; intro _ x_in _; exact Y_sub x_in) -- maybe make seperate
-      fun n ↦ (single (encodeVar box) ⊤) (partial_ τ (at n)) -- fix this later
+      have modal : Formula.modalized (encodeVar box) (partial_ τ (equation box)) := by
+        unfold box
+        have is_box := box_in_Y.choose_spec.1
+        cases r_def : r 𝕏.α box_in_Y.choose <;> simp [r_def] at is_box <;> simp [RuleApp.isBox] at is_box
+        · unfold equation
+          split <;> simp_all
+          simp [partial_, Formula.modalized]
+        · unfold equation
+          split <;> simp_all
+          simp [partial_, Formula.modalized]
+      have ψ := (FixedPointTheorem (partial_ τ (equation box)) (encodeVar box) modal).choose-- I think this is what we want
+      fun n ↦ (single (encodeVar box) ψ) (partial_ τ (at n))
     else
       have y_in_Y : ∃ y, y ∈ Y := by by_contra h; apply em_con; apply Finset.eq_empty_of_forall_notMem; simp_all
       have leaf_in_Y := finite_and_no_loop_implies_exists_leaf (fun x ↦ x ∈ Y) y_in_Y.choose y_in_Y.choose_spec loop_con
@@ -235,7 +270,7 @@ def Solution_strong {𝕏 : Proof} [fin_X : Fintype 𝕏.X]
 
 termination_by Finset.card Y
 decreasing_by
-  · have box_in : box ∈ Y := box_in_Y.choose_spec.2
+  · have box_in : box ∈ Y := box_in_Y.choose_spec.2.1
     simp [←Finset.card_sdiff_add_card_inter Y {box}, box_in]
     linarith
   · have leaf_in : leaf ∈ Y := leaf_in_Y.choose_spec.1
@@ -244,97 +279,613 @@ decreasing_by
 
 theorem equiv_help {C D E : Formula} (h : C ≅ D) (g : D = E) : (C ≅ E) := by aesop
 
-set_option maxHeartbeats 1000000
+-- ∀ m ∈ σ (pₓ), m ∈ (l(x)) ∩ r(x)) ∪ (X / Y) p ∈ ψ [q/φ]
+
+theorem in_single_voc' {m n : ℕ} {φ ψ : Formula} : m ∈ (single n φ ψ).vocab → (m ∈ φ.vocab ∧ n ∈ ψ.vocab) ∨ (m ∈ ψ.vocab ∧ m ≠ n) := by
+  intro m_in
+  induction ψ <;> simp_all [single] <;> try grind [Formula.vocab, in_neg_voc_iff, Formula.instTop, Formula.instBot]
+
+theorem in_vocab_of_path_left {𝕏 : Proof} {x y : 𝕏.X} (x_y : Relation.ReflTransGen (edge 𝕏.α) x y) {n} (n_in : n ∈ (SplitSequent.left (f (r 𝕏.α y))).vocab)
+  : n ∈ (SplitSequent.left (f (r 𝕏.α x))).vocab := by
+  induction x_y
+  case refl => exact n_in
+  case tail y z x_y y_z ih =>
+    apply ih
+    have Xh := 𝕏.h y
+    simp [SplitSequent.left, Sequent.vocab] at n_in
+    have ⟨φ, φ_in_f, n_in_φ⟩ := n_in
+    cases r_def : r 𝕏.α y <;> simp_all [edge] <;> simp [f, SplitSequent.left, Sequent.vocab]
+    case andₗ Δ φ₁ φ₂ in_Δ =>
+      have := @List.mem_map_of_mem _ _ _ _ (fun x ↦ f (r 𝕏.α x)) y_z
+      simp_all
+      rcases this with l | l <;> simp [l, fₙ_alternate] at φ_in_f
+      all_goals
+      · rcases φ_in_f with c1 | c2
+        · exact ⟨φ₁ & φ₂, in_Δ, by simp [Formula.vocab, c1 ▸ n_in_φ]⟩
+        · exact ⟨φ, c2.1, n_in_φ⟩
+    case andᵣ Δ φ₁ φ₂ in_Δ =>
+      have := @List.mem_map_of_mem _ _ _ _ (fun x ↦ f (r 𝕏.α x)) y_z
+      simp_all
+      rcases this with l | l <;> simp [l, fₙ_alternate] at φ_in_f
+      all_goals
+        exact ⟨φ, φ_in_f, n_in_φ⟩
+    case orₗ Δ φ₁ φ₂ in_Δ =>
+      have ⟨z, _, f_eq⟩ := Xh
+      simp_all [fₙ_alternate]
+      subst y_z
+      rcases φ_in_f with c1 | c2 | c3
+      · exact ⟨φ₁ v φ₂, in_Δ, by simp [Formula.vocab, c1 ▸ n_in_φ]⟩
+      · exact ⟨φ₁ v φ₂, in_Δ, by simp [Formula.vocab, c2 ▸ n_in_φ]⟩
+      · exact ⟨φ, c3.1, n_in_φ⟩
+    case orᵣ Δ φ₁ φ₂ in_Δ =>
+      have ⟨z, _, f_eq⟩ := Xh
+      simp_all [fₙ_alternate]
+    case boxₗ Δ φ₁ in_Δ =>
+      have ⟨z, _, f_eq⟩ := Xh
+      simp_all [fₙ_alternate, SplitSequent.D]
+      subst y_z
+      rcases φ_in_f with c1 | c2 | c3
+      · exact ⟨□φ₁, in_Δ, by simp [Formula.vocab, c1 ▸ n_in_φ]⟩
+      · exact ⟨φ, c2.1.1, n_in_φ⟩
+      · exact ⟨◇φ, c3, by simp [Formula.vocab, n_in_φ]⟩
+    case boxᵣ Δ φ₁ in_Δ =>
+      have ⟨z, _, f_eq⟩ := Xh
+      simp_all [fₙ_alternate, SplitSequent.D]
+      rcases φ_in_f with c1 | c2
+      · exact ⟨φ, c1.1, n_in_φ⟩
+      · exact ⟨◇φ, c2, by simp [Formula.vocab, n_in_φ]⟩
+
+theorem in_vocab_of_path_right {𝕏 : Proof} {x y : 𝕏.X} (x_y : Relation.ReflTransGen (edge 𝕏.α) x y) {n} (n_in : n ∈ (SplitSequent.right (f (r 𝕏.α y))).vocab)
+  : n ∈ (SplitSequent.right (f (r 𝕏.α x))).vocab := by
+  induction x_y
+  case refl => exact n_in
+  case tail y z x_y y_z ih =>
+    apply ih
+    have Xh := 𝕏.h y
+    simp [SplitSequent.right, Sequent.vocab] at n_in
+    have ⟨φ, φ_in_f, n_in_φ⟩ := n_in
+    cases r_def : r 𝕏.α y <;> simp_all [edge] <;> simp [f, SplitSequent.right, Sequent.vocab]
+    case andᵣ Δ φ₁ φ₂ in_Δ =>
+      have := @List.mem_map_of_mem _ _ _ _ (fun x ↦ f (r 𝕏.α x)) y_z
+      simp_all
+      rcases this with l | l <;> simp [l, fₙ_alternate] at φ_in_f
+      all_goals
+      · rcases φ_in_f with c1 | c2
+        · exact ⟨φ₁ & φ₂, in_Δ, by simp [Formula.vocab, c1 ▸ n_in_φ]⟩
+        · exact ⟨φ, c2.1, n_in_φ⟩
+    case andₗ Δ φ₁ φ₂ in_Δ =>
+      have := @List.mem_map_of_mem _ _ _ _ (fun x ↦ f (r 𝕏.α x)) y_z
+      simp_all
+      rcases this with l | l <;> simp [l, fₙ_alternate] at φ_in_f
+      all_goals
+        exact ⟨φ, φ_in_f, n_in_φ⟩
+    case orᵣ Δ φ₁ φ₂ in_Δ =>
+      have ⟨z, _, f_eq⟩ := Xh
+      simp_all [fₙ_alternate]
+      subst y_z
+      rcases φ_in_f with c1 | c2 | c3
+      · exact ⟨φ₁ v φ₂, in_Δ, by simp [Formula.vocab, c1 ▸ n_in_φ]⟩
+      · exact ⟨φ₁ v φ₂, in_Δ, by simp [Formula.vocab, c2 ▸ n_in_φ]⟩
+      · exact ⟨φ, c3.1, n_in_φ⟩
+    case orₗ Δ φ₁ φ₂ in_Δ =>
+      have ⟨z, _, f_eq⟩ := Xh
+      simp_all [fₙ_alternate]
+    case boxᵣ Δ φ₁ in_Δ =>
+      have ⟨z, _, f_eq⟩ := Xh
+      simp_all [fₙ_alternate, SplitSequent.D]
+      subst y_z
+      rcases φ_in_f with c1 | c2 | c3
+      · exact ⟨□φ₁, in_Δ, by simp [Formula.vocab, c1 ▸ n_in_φ]⟩
+      · exact ⟨φ, c2.1.1, n_in_φ⟩
+      · exact ⟨◇φ, c3, by simp [Formula.vocab, n_in_φ]⟩
+    case boxₗ Δ φ₁ in_Δ =>
+      have ⟨z, _, f_eq⟩ := Xh
+      simp_all [fₙ_alternate, SplitSequent.D]
+      rcases φ_in_f with c1 | c2
+      · exact ⟨φ, c1.1, n_in_φ⟩
+      · exact ⟨◇φ, c2, by simp [Formula.vocab, n_in_φ]⟩
+
+theorem encodeVar_eq {𝕏 : Proof} {Fin_X : Fintype 𝕏.X} {x : 𝕏.X} {n : ℕ} {h1} {h2 : n ≥ 𝕏.freeVar} : encodeVar x = n ↔ x = unencodeVar n h1 := by
+  constructor
+  · intro mp
+    subst mp
+    simp [encodeVar_inv]
+  · intro mpp
+    subst mpp
+    apply unencodeVar_inv
+    exact h2
+
+set_option maxHeartbeats 1000000 in
 open Classical in
-theorem Solution_strong_prop' {𝕏 : Proof} [fin_X : Fintype 𝕏.X]
+theorem Solution_strong_prop {𝕏 : Proof} [fin_X : Fintype 𝕏.X]
   (Y : Finset 𝕏.X) (Y_sub : Y ⊆ fin_X.elems) :
       ∀ n : {n // n ∈ Y.image encodeVar},
           ((Solution_strong Y_sub n = partial_ (Solution_strong Y_sub) (equation (unencodeVar n (helper_1 n.2))))
          ∨ (Solution_strong Y_sub n ≅ partial_ (Solution_strong Y_sub) (equation (unencodeVar n (helper_1 n.2)))))
-       ∧ (∀ m : {m // m ∈ Y.image encodeVar}, m.1 ∉ (Solution_strong Y_sub n).vocab) := by
-
-  intro ⟨n, n_in⟩
+       ∧ (∀ m ∈ (Solution_strong Y_sub n).vocab, m ∈ ((SplitSequent.left (f (r 𝕏.α (unencodeVar n (helper_1 n.2))))).vocab ∩ (SplitSequent.right (f (r 𝕏.α (unencodeVar n (helper_1 n.2))))).vocab) ∪ (fin_X.elems.image encodeVar \ Y.image encodeVar))
+       ∧ (∀ y : 𝕏.X, encodeVar y ∈ (partial_ (Solution_strong Y_sub) (at n)).vocab → (Relation.ReflTransGen (edge 𝕏.α)) (unencodeVar n (helper_1 n.2)) y)
+       := by
   unfold Solution_strong
+  intro ⟨n, n_in⟩
   by_cases em_con : Y = ∅
   · subst em_con
     simp at n_in
   · by_cases loop_con : ∃ y, Relation.TransGen (edge_restr (fun x ↦ x ∈ Y)) y y
     case pos =>
       simp [em_con, loop_con]
-      sorry
+      have box_in_Y := exists_box_on_restr_loop loop_con.choose (fun x ↦ x ∈ Y) loop_con.choose_spec
+      have Z_sub : Y \ {box_in_Y.choose} ⊆ Fintype.elems := by simp [Finset.subset_iff]; intro _ x_in _; exact Y_sub x_in
+      let τ_prop := @Solution_strong_prop _ _ (Y \ {box_in_Y.choose}) Z_sub -- maybe make seperate
+      have modal : Formula.modalized (encodeVar box_in_Y.choose) (partial_ (Solution_strong Z_sub) (equation box_in_Y.choose)) := by
+        have is_box := box_in_Y.choose_spec.1
+        cases r_def : r 𝕏.α box_in_Y.choose <;> simp [r_def] at is_box <;> simp [RuleApp.isBox] at is_box
+        · unfold equation
+          split <;> simp_all
+          simp [partial_, Formula.modalized]
+        · unfold equation
+          split <;> simp_all
+          simp [partial_, Formula.modalized]
+      have fpt := FixedPointTheorem (partial_ (Solution_strong Z_sub) (equation box_in_Y.choose)) (encodeVar box_in_Y.choose) modal
+      have const := partial_const (Solution_strong Z_sub) (at (encodeVar box_in_Y.choose)) (by
+        simp [Formula.vocab, Finset.mem_singleton, forall_eq])
+      have ⟨z, p_eq, z_in, box_z⟩ : ∃ z, p 𝕏.α box_in_Y.choose = [z] ∧ z ∈ Y ∧ z ∈ p 𝕏.α box_in_Y.choose := by
+        have is_box := box_in_Y.choose_spec.1
+        have Xh := 𝕏.h box_in_Y.choose
+        cases r_def : r 𝕏.α box_in_Y.choose <;> simp [r_def] at is_box <;> simp [RuleApp.isBox] at is_box <;> simp [r_def] at Xh
+        all_goals
+        refine ⟨Xh.choose, Xh.choose_spec.1, ?_, ?_⟩
+        · by_cases box_is_z : box_in_Y.choose = Xh.choose
+          · simp [←box_is_z]
+            exact box_in_Y.choose_spec.2.1
+          · have ⟨d, box_d⟩ : ∃ d, Relation.TransGen (edge_restr fun x ↦ x ∈ Y) box_in_Y.choose d := by
+              exact ⟨box_in_Y.choose, box_in_Y.choose_spec.2.2⟩
+            cases box_d using Relation.TransGen.head_induction_on
+            case neg.single box_d =>
+              unfold edge_restr edge at box_d
+              convert box_d.2.2
+              have := Xh.choose_spec.1
+              rw [this] at box_d
+              exact Eq.symm $ List.mem_singleton.1 box_d.1
+            case neg.head box_d heq =>
+              unfold edge_restr edge at box_d
+              convert box_d.2.2
+              have := Xh.choose_spec.1
+              rw [this] at box_d
+              exact Eq.symm $ List.mem_singleton.1 box_d.1
+        · have := Xh.choose_spec.1
+          convert List.mem_singleton_self Xh.choose
+      have equation_eq : equation box_in_Y.choose = □ (at (encodeVar z)) ∨ equation box_in_Y.choose = ◇ (at (encodeVar z)) := by
+        have is_box := box_in_Y.choose_spec.1
+        unfold equation
+        split <;> rename_i r_def <;> simp [r_def] at is_box <;> simp [RuleApp.isBox] at is_box <;> simp [p_eq]
+      by_cases n = encodeVar box_in_Y.choose
+      case pos y_eq_box =>
+        subst y_eq_box
+        refine ⟨?_, ?_, ?_⟩
+        · right -- double check this
+          simp [partial_, single, encodeVar_inv]
+          have h : fpt.choose ≅ (single (encodeVar box_in_Y.choose) fpt.choose (partial_ (Solution_strong Z_sub) (equation box_in_Y.choose))) := by sorry
+          convert h using 1
+          rcases equation_eq with c | c
+          all_goals
+            simp [c, partial_, single, z_in]
+        · simp [←const, single]
+          intro m m_in_fpt
+          have m_in_eq := fpt.choose_spec.2.2 m_in_fpt
+          rcases equation_eq with c | c
+          all_goals
+            simp [c, partial_, Formula.vocab] at m_in_eq
+            by_cases box_is_z : z = box_in_Y.choose
+            · exfalso
+              subst box_is_z
+              simp [Formula.vocab] at m_in_eq
+              subst m_in_eq
+              exact fpt.choose_spec.1 m_in_fpt
+            · simp [z_in, box_is_z] at m_in_eq
+              have m_in_ih := (τ_prop ⟨encodeVar z, by simp [z_in, box_is_z]⟩).2.1 _ m_in_eq
+              simp at m_in_ih
+              rcases m_in_ih with m_in_seq | m_in_var
+              · refine Or.inl ⟨?_, ?_⟩
+                · convert @in_vocab_of_path_left 𝕏 box_in_Y.choose z (Relation.ReflTransGen.single box_z) m (by convert m_in_seq.1; simp [encodeVar_inv])
+                  simp [encodeVar_inv]
+                · convert @in_vocab_of_path_right 𝕏 box_in_Y.choose z (Relation.ReflTransGen.single box_z) m (by convert m_in_seq.2; simp [encodeVar_inv])
+                  simp [encodeVar_inv]
+              · refine Or.inr ⟨m_in_var.1, ?_⟩
+                · intro x x_in con
+                  subst con
+                  apply m_in_var.2 x x_in
+                  intro con
+                  subst con
+                  apply fpt.choose_spec.1 m_in_fpt
+                  rfl
+        · intro y
+          simp [partial_, single, n_in, encodeVar_inv]
+          intro mp
+          have mp := fpt.choose_spec.2.2 mp
+          rcases equation_eq with c | c
+          all_goals
+            by_cases box_is_z : z = box_in_Y.choose
+            · subst box_is_z
+              simp [c, partial_, Formula.vocab] at mp
+              subst mp
+              exact Relation.ReflTransGen.refl
+            · simp [c, partial_, Formula.vocab, z_in, box_is_z] at mp
+              have z_y := (τ_prop ⟨encodeVar z, by simp_all⟩).2.2 y (by convert mp; simp [partial_, z_in, box_is_z])
+              simp [encodeVar_inv] at z_y
+              apply Relation.ReflTransGen.head box_z z_y
+      case neg y_ne_box =>
+        have n_in' : n ∈ Finset.image encodeVar (Y \ {box_in_Y.choose}) := by
+          simp only [Finset.mem_image, Finset.mem_sdiff, Finset.mem_singleton]
+          refine ⟨unencodeVar n (helper_1 n_in), ⟨helper_2 n_in, ?_⟩, ?_⟩
+          · intro con
+            apply y_ne_box
+            simp [←con, encodeVar, unencodeVar]
+            have := helper_1 n_in
+            simp at n_in
+            have ⟨y, y_in, y_eq⟩ := n_in
+            subst y_eq
+            simp [encodeVar]
+          · apply unencodeVar_inv
+            simp at n_in
+            have ⟨y, y_in, y_eq⟩ := n_in
+            subst y_eq
+            simp [encodeVar]
+        have ⟨eq_or_equiv, vocab, path⟩ := τ_prop ⟨n, n_in'⟩
+        refine ⟨?_, ?_, ?_⟩
+        · rcases eq_or_equiv with eq | equiv
+          · left
+            simp [partial_, n_in', eq]
+            convert @Solution_strong_helper _ _ (Solution_strong Z_sub) (encodeVar box_in_Y.choose) fpt.choose (equation (unencodeVar n (helper_1 n_in)))
+            · simp
+              constructor
+              · intro ⟨y, y_in, y_eq⟩
+                subst y_eq
+                by_cases y_is_box : y = box_in_Y.choose
+                · subst y_is_box
+                  right
+                  rfl
+                · left
+                  use y
+              · intro mpp
+                rcases mpp with ⟨y, ⟨y_in, y_not_box⟩, y_eq⟩ | x_eq
+                · subst y_eq
+                  use y
+                · subst x_eq
+                  exact ⟨box_in_Y.choose, box_in_Y.choose_spec.2.1, rfl⟩
+            · simp
+              rename_i heq
+              constructor
+              · intro mpp
+                have ⟨y, ⟨y_in, y_not_box⟩, y_eq⟩ := mpp
+                refine ⟨y, ⟨y_in, y_not_box⟩, ?_⟩
+                convert y_eq
+                · simp
+                  constructor
+                  · intro mp
+                    rcases mp with l | r
+                    · exact ⟨l.choose, l.choose_spec.1.1, l.choose_spec.2⟩
+                    · exact ⟨box_in_Y.choose, box_in_Y.choose_spec.2.1, Eq.symm r⟩
+                  · intro mpp
+                    have ⟨y, y_in_Y, y_eq⟩ := mpp
+                    subst y_eq
+                    by_cases h : y = box_in_Y.choose
+                    · right
+                      subst h
+                      rfl
+                    · left
+                      use y
+                · exact HEq.symm heq
+              · intro mp
+                have ⟨y, ⟨y_in, y_not_box⟩, y_eq⟩ := mp
+                refine ⟨y, ⟨y_in, y_not_box⟩, ?_⟩
+                convert y_eq
+          · right
+            simp [partial_, n_in']
+            have := single_preserves_equiv (encodeVar box_in_Y.choose) fpt.choose _ _ equiv
+            apply equiv_help this
 
+            convert @Solution_strong_helper _ _ (Solution_strong Z_sub) (encodeVar box_in_Y.choose) fpt.choose (equation (unencodeVar n (helper_1 n_in)))
+            · simp
+              constructor
+              · intro mp
+                have ⟨y, y_in_Y, y_eq⟩ := mp
+                subst y_eq
+                by_cases h : y = box_in_Y.choose
+                · right
+                  subst h
+                  rfl
+                · left
+                  use y
+              · intro mpp
+                rcases mpp with l | r
+                · exact ⟨l.choose, l.choose_spec.1.1, l.choose_spec.2⟩
+                · exact ⟨box_in_Y.choose, box_in_Y.choose_spec.2.1, Eq.symm r⟩
+            · simp
+              rename_i heq
+              constructor
+              · intro mpp
+                have ⟨y, ⟨y_in, y_not_box⟩, y_eq⟩ := mpp
+                refine ⟨y, ⟨y_in, y_not_box⟩, ?_⟩
+                convert y_eq
+                · simp
+                  constructor
+                  · intro mp
+                    rcases mp with l | r
+                    · exact ⟨l.choose, l.choose_spec.1.1, l.choose_spec.2⟩
+                    · exact ⟨box_in_Y.choose, box_in_Y.choose_spec.2.1, Eq.symm r⟩
+                  · intro mpp
+                    have ⟨y, y_in_Y, y_eq⟩ := mpp
+                    subst y_eq
+                    by_cases h : y = box_in_Y.choose
+                    · right
+                      subst h
+                      rfl
+                    · left
+                      use y
+                · exact HEq.symm heq
+              · intro mp
+                have ⟨y, ⟨y_in, y_not_box⟩, y_eq⟩ := mp
+                refine ⟨y, ⟨y_in, y_not_box⟩, ?_⟩
+                convert y_eq
+        · intro m m_in
+          rcases in_single_voc' m_in with ⟨m_in_fpt, box_in_τ⟩ | ⟨m_in_τ, m_not_box⟩
+          · have m_in_eq := fpt.choose_spec.2.2 m_in_fpt
+            rcases equation_eq with c | c
+            all_goals
+            by_cases z_is_box : z = box_in_Y.choose
+            · exfalso
+              simp [c, partial_, Formula.vocab, z_is_box] at m_in_eq
+              subst m_in_eq
+              apply fpt.choose_spec.1
+              exact m_in_fpt
+            · simp [partial_, n_in'] at m_in
+              simp [c, partial_, Formula.vocab, z_is_box, z_in] at m_in_eq
+              have m_in := (τ_prop ⟨encodeVar z, by simp [z_in, z_is_box]⟩).2.1 m m_in_eq
+              simp at m_in
+              rcases m_in with m_in_seq | m_in_var
+              · refine Or.inl ⟨?_, ?_⟩
+                · apply @in_vocab_of_path_left 𝕏 (unencodeVar n (helper_1 n_in)) z ?_ m (by convert m_in_seq.1; simp [encodeVar_inv])
+                  exact Relation.ReflTransGen.tail (path box_in_Y.choose box_in_τ) box_z
+                · apply @in_vocab_of_path_right 𝕏 (unencodeVar n (helper_1 n_in)) z ?_ m (by convert m_in_seq.2; simp [encodeVar_inv])
+                  exact Relation.ReflTransGen.tail (path box_in_Y.choose box_in_τ) box_z
+              · refine Or.inr ⟨m_in_var.1, ?_⟩
+                · intro x x_in con
+                  subst con
+                  apply m_in_var.2 x x_in
+                  intro con
+                  subst con
+                  apply fpt.choose_spec.1 m_in_fpt
+                  rfl
+          · simp [partial_, n_in'] at m_in_τ
+            have ih := vocab m m_in_τ
+            simp at ih
+            rcases ih with ih1 | ih2
+            · exact Or.inl ih1
+            · refine Or.inr ⟨ih2.1, ?_⟩
+              intro x x_in con
+              apply ih2.2 x x_in ?_ con
+              intro eq
+              subst eq
+              subst con
+              apply m_not_box
+              rfl
+        · simp [partial_, n_in, n_in']
+          simp [partial_, n_in'] at path
+          intro y mp
+          rcases in_single_voc' mp with ⟨y_in_fpt, box_in_τ⟩ | ⟨y_in_τ, y_not_box⟩
+          · have y_in_eq := fpt.choose_spec.2.2 y_in_fpt
+            rcases equation_eq with c | c
+            all_goals
+              simp [c, partial_, Formula.vocab, z_in] at y_in_eq
+              by_cases z_is_box : z = box_in_Y.choose
+              · subst z_is_box
+                simp [Formula.vocab] at y_in_eq
+                subst y_in_eq
+                exact path box_in_Y.choose box_in_τ
+              · simp [z_is_box] at y_in_eq
+                have := (τ_prop ⟨encodeVar z, by simp [z_in, z_is_box]⟩).2.2
+                simp [partial_, z_in, z_is_box, encodeVar_inv] at this
+                apply Relation.ReflTransGen.trans ?_ (this y y_in_eq)
+                exact Relation.ReflTransGen.tail (path box_in_Y.choose box_in_τ) box_z
+          · exact path y y_in_τ
     case neg =>
       simp [em_con, loop_con]
       have y_in_Y : ∃ y, y ∈ Y := by by_contra h; apply em_con; apply Finset.eq_empty_of_forall_notMem; simp_all
       have leaf_in_Y := finite_and_no_loop_implies_exists_leaf (fun x ↦ x ∈ Y) y_in_Y.choose y_in_Y.choose_spec loop_con
+      have Z_sub : Y \ {leaf_in_Y.choose} ⊆ Fintype.elems := by simp [Finset.subset_iff]; intro _ x_in _; exact Y_sub x_in
+      let τ_prop := @Solution_strong_prop _ _ (Y \ {leaf_in_Y.choose}) Z_sub -- maybe make seperate
 
-      let τ_prop := @Solution_strong_prop' _ _ (Y \ {leaf_in_Y.choose}) (by simp [Finset.subset_iff]; intro _ x_in _; exact Y_sub x_in) -- maybe make seperate
-
-      have helper : ¬ encodeVar leaf_in_Y.choose ∈ Finset.image encodeVar (Y \ {leaf_in_Y.choose}) := by
-        simp
-        intro x x_in hyp con
-        apply hyp
-        exact encodeVar_inj 𝕏 con
+      have const := partial_const (Solution_strong Z_sub) (at (encodeVar leaf_in_Y.choose)) (by
+        simp [Formula.vocab, Finset.mem_singleton, forall_eq])
 
       by_cases n = encodeVar leaf_in_Y.choose
-      case pos y_eq_leaf =>
-        subst y_eq_leaf
-        simp [partial_, helper, single, encodeVar_inv]
-        refine ⟨Or.inl ?_, ?_⟩
-        · apply partial_const
+      case pos y_eq_box =>
+        subst y_eq_box
+        refine ⟨?_, ?_, ?_⟩
+        · left
+          simp [partial_, single, encodeVar_inv]
+          apply partial_const
           intro n n_in
           by_contra h
           simp at h
           have ⟨z, z_prop⟩ := h
           rw [←z_prop.2] at n_in
-          have y_z := encodeVar_in_equation_imp_pred n_in
+          have y_z := encodeVar_in_equation_imp_edge n_in
           exact leaf_in_Y.choose_spec.2 _ y_z z_prop.1
-        · intro z z_in con
-          exact leaf_in_Y.choose_spec.2 z (encodeVar_in_equation_imp_pred con) z_in
-      case neg y_ne_leaf =>
-        have helper : n ∈ Finset.image encodeVar (Y \ {leaf_in_Y.choose}) := by
-          simp
-          simp at n_in
-          have ⟨n, n_prop⟩ := n_in
-          refine ⟨n, ⟨n_prop.1, ?_⟩, n_prop.2⟩
-          intro con
-          rw [←con] at y_ne_leaf
-          exact y_ne_leaf (Eq.symm n_prop.2)
-        simp [partial_, helper]
-        have ⟨eq_or_equiv, sub_prop⟩ := τ_prop ⟨n, by aesop⟩
-        refine ⟨?_, ?_⟩
+
+        · simp [←const, single]
+          intro m m_in_eq
+          rcases var_in_equation _ m_in_eq with ax_or | desc
+          · left
+            simp at ax_or
+            have convert_helper := encodeVar_inv 𝕏 leaf_in_Y.choose
+            convert ax_or
+          · right
+            have ⟨y, y_eq, box_y⟩ := desc
+            subst y_eq
+            refine ⟨⟨y, fin_X.complete y, rfl⟩, ?_⟩
+            intro x x_in eq
+            have := @encodeVar_inj 𝕏 fin_X x y eq
+            subst this
+            exact leaf_in_Y.choose_spec.2 x box_y x_in
+        · intro y
+          simp [partial_, single, n_in]
+          intro mp
+          convert Relation.ReflTransGen.single (encodeVar_in_equation_imp_edge mp)
+          simp [encodeVar_inv]
+      case neg y_ne_box =>
+        have n_in' : n ∈ Finset.image encodeVar (Y \ {leaf_in_Y.choose}) := by
+          simp only [Finset.mem_image, Finset.mem_sdiff, Finset.mem_singleton]
+          refine ⟨unencodeVar n (helper_1 n_in), ⟨helper_2 n_in, ?_⟩, ?_⟩
+          · intro con
+            apply y_ne_box
+            simp [←con, encodeVar, unencodeVar]
+            have := helper_1 n_in
+            simp at n_in
+            have ⟨y, y_in, y_eq⟩ := n_in
+            subst y_eq
+            simp [encodeVar]
+          · apply unencodeVar_inv
+            simp at n_in
+            have ⟨y, y_in, y_eq⟩ := n_in
+            subst y_eq
+            simp [encodeVar]
+        have ⟨eq_or_equiv, vocab, path⟩ := τ_prop ⟨n, n_in'⟩
+        refine ⟨?_, ?_, ?_⟩
         · rcases eq_or_equiv with eq | equiv
           · left
-            convert @Solution_strong_helper (fun n ↦ n ∈ Finset.image encodeVar (Y \ {leaf_in_Y.choose})) _ (@Solution_strong _ _ (Y \ {leaf_in_Y.choose}) (by simp [Finset.subset_iff]; intro _ x_in _; exact Y_sub x_in)) (encodeVar leaf_in_Y.choose) (equation leaf_in_Y.choose) (equation (unencodeVar n (helper_1 n_in)))
-            · simp only [Finset.image_sdiff _ _ (encodeVar_inj 𝕏), Finset.mem_sdiff, Finset.image_singleton, Finset.not_mem_singleton]
-              refine ⟨by tauto, ?_⟩
-              intro h
-              rcases h with h | h <;> simp_all
-              exact ⟨leaf_in_Y.choose, leaf_in_Y.choose_spec.1, rfl⟩
-            · sorry
+            simp [partial_, n_in', eq]
+            convert @Solution_strong_helper _ _ (Solution_strong Z_sub) (encodeVar leaf_in_Y.choose) (equation leaf_in_Y.choose) (equation (unencodeVar n (helper_1 n_in)))
+            · simp
+              constructor
+              · intro mp
+                have ⟨y, y_in_Y, y_eq⟩ := mp
+                subst y_eq
+                by_cases h : y = leaf_in_Y.choose
+                · right
+                  subst h
+                  rfl
+                · left
+                  use y
+              · intro mpp
+                rcases mpp with l | r
+                · exact ⟨l.choose, l.choose_spec.1.1, l.choose_spec.2⟩
+                · exact ⟨leaf_in_Y.choose, leaf_in_Y.choose_spec.1, Eq.symm r⟩
+            · simp
+              rename_i heq
+              constructor
+              · intro mpp
+                have ⟨y, ⟨y_in, y_not_box⟩, y_eq⟩ := mpp
+                refine ⟨y, ⟨y_in, y_not_box⟩, ?_⟩
+                convert y_eq
+                · simp
+                  constructor
+                  · intro mp
+                    rcases mp with l | r
+                    · exact ⟨l.choose, l.choose_spec.1.1, l.choose_spec.2⟩
+                    · exact ⟨leaf_in_Y.choose, leaf_in_Y.choose_spec.1, Eq.symm r⟩
+                  · intro mpp
+                    have ⟨y, y_in_Y, y_eq⟩ := mpp
+                    subst y_eq
+                    by_cases h : y = leaf_in_Y.choose
+                    · right
+                      subst h
+                      rfl
+                    · left
+                      use y
+                · exact HEq.symm heq
+              · intro mp
+                have ⟨y, ⟨y_in, y_not_box⟩, y_eq⟩ := mp
+                refine ⟨y, ⟨y_in, y_not_box⟩, ?_⟩
+                convert y_eq
           · right
+            simp [partial_, n_in']
             have := single_preserves_equiv (encodeVar leaf_in_Y.choose) (equation leaf_in_Y.choose) _ _ equiv
             apply equiv_help this
-            convert @Solution_strong_helper (fun n ↦ n ∈ Finset.image encodeVar (Y \ {leaf_in_Y.choose})) _ (@Solution_strong _ _ (Y \ {leaf_in_Y.choose}) (by simp [Finset.subset_iff]; intro _ x_in _; exact Y_sub x_in)) (encodeVar leaf_in_Y.choose) (equation leaf_in_Y.choose) (equation (unencodeVar n (helper_1 n_in)))
-            · simp only [Finset.image_sdiff _ _ (encodeVar_inj 𝕏), Finset.mem_sdiff, Finset.image_singleton, Finset.not_mem_singleton]
-              refine ⟨by tauto, ?_⟩
-              intro h
-              rcases h with h | h <;> simp_all
-              exact ⟨leaf_in_Y.choose, leaf_in_Y.choose_spec.1, rfl⟩
-            · sorry
-        · intro z z_in
-          apply in_single_voc
-          · intro con
-            exact leaf_in_Y.choose_spec.2 z (encodeVar_in_equation_imp_pred con) z_in
-          · intro not_leaf
-            exact sub_prop ⟨encodeVar z, by aesop⟩
-          · intro con
-            exact leaf_in_Y.choose_spec.2 leaf_in_Y.choose (encodeVar_in_equation_imp_pred con) leaf_in_Y.choose_spec.1
 
+            convert @Solution_strong_helper _ _ (Solution_strong Z_sub) (encodeVar leaf_in_Y.choose) (equation leaf_in_Y.choose) (equation (unencodeVar n (helper_1 n_in)))
+            · simp
+              constructor
+              · intro mp
+                have ⟨y, y_in_Y, y_eq⟩ := mp
+                subst y_eq
+                by_cases h : y = leaf_in_Y.choose
+                · right
+                  subst h
+                  rfl
+                · left
+                  use y
+              · intro mpp
+                rcases mpp with l | r
+                · exact ⟨l.choose, l.choose_spec.1.1, l.choose_spec.2⟩
+                · exact ⟨leaf_in_Y.choose, leaf_in_Y.choose_spec.1, Eq.symm r⟩
+            · simp
+              rename_i heq
+              constructor
+              · intro mpp
+                have ⟨y, ⟨y_in, y_not_box⟩, y_eq⟩ := mpp
+                refine ⟨y, ⟨y_in, y_not_box⟩, ?_⟩
+                convert y_eq
+                · simp
+                  constructor
+                  · intro mp
+                    rcases mp with l | r
+                    · exact ⟨l.choose, l.choose_spec.1.1, l.choose_spec.2⟩
+                    · exact ⟨leaf_in_Y.choose, leaf_in_Y.choose_spec.1, Eq.symm r⟩
+                  · intro mpp
+                    have ⟨y, y_in_Y, y_eq⟩ := mpp
+                    subst y_eq
+                    by_cases h : y = leaf_in_Y.choose
+                    · right
+                      subst h
+                      rfl
+                    · left
+                      use y
+                · exact HEq.symm heq
+              · intro mp
+                have ⟨y, ⟨y_in, y_not_box⟩, y_eq⟩ := mp
+                refine ⟨y, ⟨y_in, y_not_box⟩, ?_⟩
+                convert y_eq
+
+        · intro m m_in
+          rcases in_single_voc' m_in with ⟨m_in_eq, leaf_in_τ⟩ | ⟨m_in_τ, m_not_box⟩
+          · rcases var_in_equation _ m_in_eq with ax_or | desc
+            · left
+              have un_y := path leaf_in_Y.choose leaf_in_τ
+              simp at ax_or
+              exact ⟨in_vocab_of_path_left un_y ax_or.1, in_vocab_of_path_right un_y ax_or.2⟩
+            · right
+              have ⟨y, y_eq, leaf_y⟩ := desc
+              subst y_eq
+              refine ⟨⟨y, fin_X.complete y, rfl⟩, ?_⟩
+              intro x x_in eq
+              have := @encodeVar_inj 𝕏 fin_X x y eq
+              subst this
+              exact leaf_in_Y.choose_spec.2 x leaf_y x_in
+          · simp [partial_, n_in'] at m_in_τ
+            have ih := vocab m m_in_τ
+            simp at ih
+            rcases ih with ih1 | ih2
+            · exact Or.inl ih1
+            · refine Or.inr ⟨ih2.1, ?_⟩
+              intro x x_in con
+              apply ih2.2 x x_in ?_ con
+              intro eq
+              subst eq
+              subst con
+              apply m_not_box
+              rfl
+        · simp [partial_, n_in, n_in']
+          simp [partial_, n_in'] at path
+          intro y mp
+          rcases in_single_voc' mp with ⟨y_in_eq, leaf_in_τ⟩ | ⟨y_in_τ, y_not_box⟩
+          · exact Relation.ReflTransGen.tail (path leaf_in_Y.choose leaf_in_τ) (encodeVar_in_equation_imp_edge y_in_eq)
+          · exact path y y_in_τ
 termination_by Finset.card Y
 decreasing_by
-  all_goals
-    have leaf_in := leaf_in_Y.choose_spec.1
+  · have box_in : box_in_Y.choose ∈ Y := box_in_Y.choose_spec.2.1
+    simp [←Finset.card_sdiff_add_card_inter Y {box_in_Y.choose}, box_in]
+  · have leaf_in : leaf_in_Y.choose ∈ Y := leaf_in_Y.choose_spec.1
     simp [←Finset.card_sdiff_add_card_inter Y {leaf_in_Y.choose}, leaf_in]
 
 noncomputable def Interpolant (𝕏 : Proof) [fin_X : Fintype 𝕏.X] : Formula → Formula
@@ -347,11 +898,11 @@ by
 theorem Interpolant_prop {𝕏 : Proof} [fin_X : Fintype 𝕏.X] (x : 𝕏.X) :
     (Interpolant 𝕏 (at (encodeVar x)) = Interpolant 𝕏 (equation x)
   ∨ (Interpolant 𝕏 (at (encodeVar x)) ≅ Interpolant 𝕏 (equation x)))
-  ∧ (∀ y : 𝕏.X, encodeVar y ∉ (Interpolant 𝕏 (at (encodeVar x))).vocab)
+  ∧ (Interpolant 𝕏 (at (encodeVar x))).vocab ⊆ ((SplitSequent.left (f (r 𝕏.α x))).vocab ∩ (SplitSequent.right (f (r 𝕏.α x))).vocab)
  := by
   unfold Interpolant
   have h : ∀ y : 𝕏.X, encodeVar y ∈ Finset.image encodeVar fin_X.elems := by simp [Fintype.complete]
-  have := @Solution_strong_prop' 𝕏 _ fin_X.elems (by aesop) ⟨encodeVar x, by simp [h]⟩
+  have := @Solution_strong_prop 𝕏 _ fin_X.elems (by aesop) ⟨encodeVar x, by simp [h]⟩
   refine ⟨?_, ?_⟩
   · rcases this.1 with l | r
     · left
@@ -366,6 +917,12 @@ theorem Interpolant_prop {𝕏 : Proof} [fin_X : Fintype 𝕏.X] (x : 𝕏.X) :
       · apply congrArg₂
         · rfl
         · simp [encodeVar_inv]
-  · intro y
-    convert this.2 ⟨encodeVar y, by simp [encodeVar, Fintype.complete]⟩
+  · have h : encodeVar x ∈ Finset.image encodeVar fin_X.elems := by simp; exact fin_X.complete _
     simp [partial_, h]
+    intro m m_in
+    have := this.2.1 m m_in
+    simp at this
+    convert this
+    simp [encodeVar_inv]
+
+#axiom_blame Interpolant_prop
