GL/FixedPointTheorem.lean
@@ -1,0 +1,14 @@
+import GL.Semantics
+
+def Formula.modalized (n : Nat) : Formula → Bool
+  | ⊤ => False
+  | ⊥ => False
+  | at _ => False
+  | na _ => False
+  | φ & ψ => modalized n φ ∧ modalized n ψ
+  | φ v ψ => modalized n φ ∧ modalized n ψ
+  | □ _ => True
+  | ◇ _ => True
+
+axiom FixedPointTheorem (φ : Formula) (n : ℕ) (h : φ.modalized n) : ∃ (ψ : Formula),
+  n ∉ Formula.vocab ψ ∧ sem_equiv ψ (single n ψ φ) ∧ Formula.vocab ψ ⊆ Formula.vocab φ
