GL/Interpolation.lean
@@ -17,12 +17,18 @@ theorem Interpolation (φ ψ : Formula) : ⊨ (φ ↣ ψ) → ∃ χ, isInterpol
     simp [SplitSequent.isValid, Evaluate_sseq]
     exact φ_ψ
   have ⟨𝕏, 𝕏_proves⟩ := Split.Completeness _ φ_ψ_sseq
-  have ⟨𝕐, Fin_𝕐, y, y_prop⟩ := Split.finite_proof_of_proof 𝕏 _ 𝕏_proves
-  have Fintype_Y := @Fintype.ofFinite _ Fin_𝕐 -- maybe change the Finiteness proof to prove Fintype
+  have ⟨𝕐, fin_Y, y, y_prop⟩ := Split.finite_proof_of_proof 𝕏 _ 𝕏_proves
+  have Fintype_Y := @Fintype.ofFinite _ fin_Y -- maybe change the Finiteness proof to prove Fintype
   refine ⟨Split.Interpolant 𝕐 (at (Split.encodeVar y)), ?_, ?_, ?_⟩
-  · sorry
-  · have hl : (@Split.InterpolantProofLeft 𝕐 _) ⊢ {Sum.inl (~φ), Sum.inr (Split.Interpolant 𝕐 (at (Split.encodeVar y)))} := by sorry -- this should be the main theorem of the Partial Interpolation section
+  · have := (@Split.Interpolant_prop 𝕐 Fintype_Y y).2
+    convert this
+    · ext n
+      simp [y_prop, Split.SplitSequent.left, Sequent.vocab]
+    · ext n
+      simp [y_prop, Split.SplitSequent.right, Sequent.vocab]
+  · have hl := Split.InterpolantProofLeft_proves_interpolant y
     have φ_χ := SplitCut.Soundness _ ⟨_, hl⟩
-    simp [SplitSequent.isValid, Evaluate_sseq] at φ_χ
-    exact φ_χ
+    simp [SplitSequent.isValid, Evaluate_sseq, Split.leftInterpolantSequent, y_prop] at φ_χ
+    simp [Formula.isValid]
+    grind
   · sorry
